Setup for inode encoding/decoding

src/program_proof/simplefs/bitmap_proof.v
@@ -8,6 +8,7 @@ Import Nat.
 From Goose.github_com Require Import tchajed.simplefs.bitmap.
 
 From Perennial.program_proof.simplefs Require Import bitmap_byte.
+From Perennial.program_proof.simplefs Require Import concat.
 
 Set Default Proof Using "Type".
 
@@ -16,71 +17,6 @@ Set Default Proof Using "Type".
 
 Definition bytes_to_bits (data: list u8): list bool :=
   concat (byte_to_bits <$> data).
-
-Definition length_uniform {A: Type} (l: list (list A)) (n: nat) :=
-  ∀ i x, l !! i = Some x → length x = n.
-
-Lemma length_uniform_app_inv {A} (a: list A) (l: list (list A)) n :
-  length_uniform (a :: l) n →
-  length a = n ∧ length_uniform l n.
-Proof.
-  rewrite /length_uniform.
-  intros Hlen.
-  pose proof (Hlen 0%nat a) as H; simpl in H.
-  split; auto.
-  intros.
-  pose proof (Hlen (S i)). auto.
-Qed.
-
-Lemma length_concat_uniform {A: Type} (l: list (list A)) (n: nat) :
-  length_uniform l n →
-  length (concat l) = (length l * n)%nat.
-Proof.
-  intros Hlen.
-  induction l; simpl; auto.
-  apply length_uniform_app_inv in Hlen as [Ha Hlen].
-  intuition.
-  autorewrite with len.
-  rewrite H //.
-  lia.
-Qed.
-
-Lemma Nat_mod_add_modulus n k :
-  ((n + k) `mod` k = n `mod` k)%nat.
-Proof.
-  rewrite (Div0.add_mod n k k).
-  rewrite Div0.mod_same.
-  rewrite Nat.add_0_r.
-  rewrite Div0.mod_mod.
-  reflexivity.
-Qed.
-
-Lemma lookup_concat_uniform {A: Type} (l: list (list A)) (n: nat) :
-  length_uniform l n →
-  n ≠ 0%nat →
-  ∀ i, concat l !! i =
-         (l !! (i `div` n)%nat) ≫= λ (ll: list A), ll !! (i `mod` n)%nat.
-Proof.
-  intros Hlen Hn.
-  induction l.
-  - simpl. intros. rewrite lookup_nil //.
-  - apply length_uniform_app_inv in Hlen as [Ha Hlen].
-    simpl. intros i.
-    destruct (decide (i < n)%nat).
-    + rewrite lookup_app_l; [ | lia ].
-      rewrite Nat.div_small // /=.
-      rewrite Nat.mod_small //.
-    + rewrite lookup_app_r; [ | lia ].
-      rewrite IHl //.
-      rewrite Ha.
-      replace i with (1*n + (i-n))%nat at 2 by lia.
-      rewrite Nat.div_add_l; [ | lia ].
-      simpl.
-      f_equal.
-      f_equal.
-      rewrite -(Nat_mod_add_modulus (i-n) n).
-      replace (i - n + n)%nat with i by lia; auto.
-Qed.
 
 Lemma bytes_to_bits_uniform block :
   length_uniform (byte_to_bits <$> block) 8%nat.
