src/program_proof/simplefs/concat.v
@@ -1,0 +1,91 @@
+From stdpp Require Import base list.
+From Coq Require Import ssreflect.
+
+From Perennial.Helpers Require Import NatDivMod Integers Tactics.
+
+Local Open Scope Z.
+
+#[local] Ltac Zify.zify_post_hook ::= Z.div_mod_to_equations.
+
+Set SsrOldRewriteGoalsOrder.
+
+Definition length_uniform {A: Type} (l: list (list A)) (n: nat) :=
+  ∀ i x, l !! i = Some x → length x = n.
+
+Lemma length_uniform_u64_le (l: list u64) : length_uniform (u64_le <$> l) 8%nat.
+Proof.
+  intros i x H.
+  fmap_Some in H.
+  rewrite u64_le_length //.
+Qed.
+
+Lemma length_uniform_u32_le (l: list u32) : length_uniform (u32_le <$> l) 4%nat.
+Proof.
+  intros i x H.
+  fmap_Some in H.
+  rewrite u32_le_length //.
+Qed.
+
+Hint Resolve length_uniform_u64_le length_uniform_u32_le : core.
+
+Lemma length_uniform_app_inv {A} (a: list A) (l: list (list A)) n :
+  length_uniform (a :: l) n →
+  length a = n ∧ length_uniform l n.
+Proof.
+  rewrite /length_uniform.
+  intros Hlen.
+  pose proof (Hlen 0%nat a) as H; simpl in H.
+  split; auto.
+  intros.
+  pose proof (Hlen (S i)). auto.
+Qed.
+
+Lemma length_concat_uniform {A: Type} (l: list (list A)) (n: nat) :
+  length_uniform l n →
+  length (concat l) = (length l * n)%nat.
+Proof.
+  intros Hlen.
+  induction l; simpl; auto.
+  apply length_uniform_app_inv in Hlen as [Ha Hlen].
+  intuition.
+  rewrite length_app.
+  rewrite H //.
+  lia.
+Qed.
+
+Lemma Nat_mod_add_modulus n k :
+  ((n + k) `mod` k = n `mod` k)%nat.
+Proof.
+  rewrite (Nat.Div0.add_mod n k k).
+  rewrite Nat.Div0.mod_same.
+  rewrite Nat.add_0_r.
+  rewrite Nat.Div0.mod_mod.
+  reflexivity.
+Qed.
+
+Lemma lookup_concat_uniform {A: Type} (l: list (list A)) (n: nat) :
+  length_uniform l n →
+  n ≠ 0%nat →
+  ∀ i, concat l !! i =
+         (l !! (i `div` n)%nat) ≫= λ (ll: list A), ll !! (i `mod` n)%nat.
+Proof.
+  intros Hlen Hn.
+  induction l.
+  - simpl. intros. rewrite lookup_nil //.
+  - apply length_uniform_app_inv in Hlen as [Ha Hlen].
+    simpl. intros i.
+    destruct (decide (i < n)%nat).
+    + rewrite lookup_app_l; [ | lia ].
+      rewrite Nat.div_small // /=.
+      rewrite Nat.mod_small //.
+    + rewrite lookup_app_r; [ | lia ].
+      rewrite IHl //.
+      rewrite Ha.
+      replace i with (1*n + (i-n))%nat at 2 by lia.
+      rewrite Nat.div_add_l; [ | lia ].
+      simpl.
+      f_equal.
+      f_equal.
+      rewrite -(Nat_mod_add_modulus (i-n) n).
+      replace (i - n + n)%nat with i by lia; auto.
+Qed.
